theories/Block.v
@@ -11,8 +11,12 @@ Definition blocks_aux (G: map_cfg) : _ -> (blk*map_cfg) := fun '(id, b) => (b, r
 
 Definition blocks (G: map_cfg): list (blk*map_cfg) := List.map (blocks_aux G) (elements G).
 
-Definition blocks_aux_sem (G0 G G': map_cfg) b :=
-  MapsTo_id b G /\ G' = (remove_id b G0) /\ wf_map_cfg G'.
+Record blocks_aux_sem (G0 G G': map_cfg) b : Prop := 
+  {
+    MT: MapsTo_id b G;
+    RM: G' = remove_id b G0;
+    WF: wf_map_cfg G'
+  }.
 
 Definition blocks_sem (G G': map_cfg) b := blocks_aux_sem G G G' b.
 
@@ -23,35 +27,36 @@ Lemma blocks_aux_correct: forall G0 G, P G0 G.
 Proof.
   intros G0 G.
   apply map_induction_min; unfold P.
-  - intros E He G' B Hwf Hwf0. split.
-    * assert (HE: elements E = []) by now apply elements_Empty. now rewrite HE.
-    * intros [HE _]. contradict HE. intro. eapply empty_mapsto_iff.
-      eapply MapsTo_m. reflexivity. reflexivity. symmetry. apply Eempty. apply He. apply H.
-  - intros G1 G2 Hrec idB B HBe HB G' A Hwf2 Hwf0. rewrite Add_add in HB. 
-    assert (HidB: B.(blk_id) = idB). {
-      apply Hwf2. eapply MapsTo_m. reflexivity. reflexivity. apply HB. now apply add_1.
+  - intros E Em G' B WFE WF0. split.
+    * assert (Enil: elements E = []) by now apply elements_Empty. now rewrite Enil.
+    * intros [MTE _ _]. contradict MTE. intro MTE. eapply empty_mapsto_iff.
+      eapply MapsTo_m. reflexivity. reflexivity. symmetry. apply Eempty. apply Em. apply MTE.
+  - intros G1 G2 REC idB B Bel EQ2 G' A WF2 WF0. rewrite Add_add in EQ2.
+    assert (BidB: B.(blk_id) = idB). {
+      apply WF2. eapply MapsTo_m. reflexivity. reflexivity. apply EQ2. now apply add_1.
     } subst.
     replace (elements G2) with ((B.(blk_id), B)::(elements G1)). 2: {
       symmetry. apply eqlistA_eq. now apply elements_Add_Below.
-    } apply Below_In in HBe.
-    split. intros [H|H]. 3: case (eq_dec A.(blk_id) B.(blk_id)); unfold eq; intros He [HMA [HRA Hwf']].
+    } apply Below_In in Bel as NIN.
+    split. intros [H|H].
+    3: case (eq_dec A.(blk_id) B.(blk_id)) as [EQ|NEQ]; [unfold eq in EQ|unfold eq in NEQ]; intros [MT2 RM0 WF'].
     * apply pair_equal_spec in H as []. subst A G'. 
     repeat split; trivial.
-      + eapply MapsTo_m. reflexivity. reflexivity. apply HB. now apply add_1.
+      + eapply MapsTo_m. reflexivity. reflexivity. apply EQ2. now apply add_1.
       + now apply remove_wf_map_cfg.
-    * apply Hrec in H as [HMA [HRA Hwf']]; trivial.
-      assert (Hne: ~ A.(blk_id)===B.(blk_id)). { 
-        intro. apply HBe. exists A. eapply MapsTo_m. 4: apply HMA. now symmetry. reflexivity. reflexivity.
+    * apply REC in H as [HM1 HR0 WF']; trivial.
+      assert (NEQ: ~ A.(blk_id)===B.(blk_id)). { 
+        intro. apply NIN. exists A. eapply MapsTo_m. 4: apply HM1. now symmetry. reflexivity. reflexivity.
       }
       repeat split;trivial.
-      + eapply MapsTo_m. reflexivity. reflexivity. apply HB. apply add_2. now apply neq_sym. trivial.
-      + eapply wf_map_cfg_add. apply HBe. eapply wf_map_cfg_eq. apply HB. trivial.
+      + eapply MapsTo_m. reflexivity. reflexivity. apply EQ2. apply add_2. now apply neq_sym. trivial.
+      + eapply wf_map_cfg_add. apply NIN. eapply wf_map_cfg_eq. apply EQ2. trivial.
     * assert (Heq: A=B). { 
-      eapply wf_map_cfg_blk. apply Hwf2. apply HMA. eapply MapsTo_m.  apply He. reflexivity. apply HB. now apply add_1.
+      eapply wf_map_cfg_blk. apply WF2. apply MT2. eapply MapsTo_m. apply EQ. reflexivity. apply EQ2. now apply add_1.
     } subst. now left.
-    * right. apply Hrec; trivial. eapply wf_map_cfg_add. apply HBe. eapply wf_map_cfg_eq. apply HB. trivial.
+    * right. apply REC; trivial. eapply wf_map_cfg_add. apply NIN. eapply wf_map_cfg_eq. apply EQ2. trivial.
       repeat split; trivial.
-      eapply add_3. apply neq_sym. apply He. eapply MapsTo_m. reflexivity. reflexivity. symmetry. apply HB. trivial.
+      eapply add_3. apply neq_sym. apply NEQ. eapply MapsTo_m. reflexivity. reflexivity. symmetry. apply EQ2. trivial.
 Qed.
 
 Lemma blocks_correct: forall G G' b, wf_map_cfg G -> ((b, G') ∈ (blocks G) <-> blocks_sem G G' b).
